Trying out all-disjoint version instead

Test/extern-soundness/ExternalInvariantsDisjoint.dfy
@@ -3,44 +3,15 @@ module ExternalInvariants {
 
   trait {:termination false} ExternallyValid {
     ghost const Repr: set<object>
-    ghost const ValidatableRepr: set<ExternallyValid>
     predicate Valid() 
       reads this, Repr 
       ensures Valid() ==> 
         && this in Repr
-        && ValidatableRepr <= Repr
-        && (forall v :: v in ValidatableRepr ==> v.Repr <= Repr)
-        && (forall v :: v in ValidatableRepr && v != this ==> this !in v.Repr)
     
     // Dummy predicate to avoid "/!\ No terms found to trigger on." warning
     predicate P() {
       true
     }
-
-    // Lemma for re-establishing the external invariant after one object
-    // has changed from valid state to another valid state. Asserts that
-    // all OTHER previously valid objects are still valid based on their
-    // IndependentValidity() lemma.
-    twostate lemma AllStillValid() 
-      requires old(AllValid(set v: ExternallyValid | allocated(v) && v.P()))
-      requires Valid()
-      requires forall o :: o !in ValidatableRepr ==> unchanged(o)
-      requires forall o :: o in ValidatableRepr ==> o.Valid()
-      ensures AllValid(set v: ExternallyValid | allocated(v) && v.P())
-    {
-      forall v: ExternallyValid | old(allocated(v)) && v.P() ensures v.Valid() {
-        IndependentValidityInductive(v, Repr);
-      }
-    }
-
-    // Lemma that must be proved for each implementing class. Usually
-    // proves itself with an empty body, provided Valid() is defined
-    // in a compatible way.
-    twostate lemma IndependentValidity()
-      requires old(Valid())
-      requires unchanged(this, Repr - ValidatableRepr)
-      requires forall v :: v in ValidatableRepr && v != this ==> v.Valid()
-      ensures Valid()
 
     // Slightly silly lemma that might go away if we tweak Dafny's heuristics a bit
     lemma AllValidMakesMeValid() 
@@ -49,33 +20,11 @@ module ExternalInvariants {
     {}
   }
 
-  twostate lemma IndependentValidityInductive(v: ExternallyValid, changed: set<object>)
-      requires old(AllValid(set v': ExternallyValid | allocated(v') && v'.P()))
-      requires forall o :: o !in changed ==> unchanged(o)
-      requires forall v': ExternallyValid :: v' in changed && v' in v.ValidatableRepr ==> v'.Valid()
-      requires allocated(v)
-      decreases v.Repr
-      ensures v.Valid()
-  {
-    assert old(v.Valid());
-    forall v': ExternallyValid | v' in v.ValidatableRepr && v' != v && old(allocated(v')) ensures v'.Valid() {
-      IndependentValidityInductive(v', changed);
-    }
-    if v !in changed {
-      v.IndependentValidity();
-    }
-  }
-
-  // This is the "external invariant". It must hold as a precondition and postcondition for
-  // every method that crosses the Dafny/external boundary, either incoming or outgoing.
-  // It assumes that the Dafny heap cannot be changed in any other way.
-  // I have to pass in the set of all objects implementing ExternallyValid since I can't pass in
-  // "the Dafny heap".
   predicate AllValid(vs: set<ExternallyValid>) 
     reads vs
     reads set v, o | v in vs && o in v.Repr :: o
   {
-    forall v :: v in vs ==> v.Valid()
+    forall v :: v in vs ==> v.Valid() && forall v, v' :: v in vs && v' in vs - {v} ==> v.Repr !! v'.Repr
   }
 
   // class NotAtomic {
